LCF.v
@@ -5,6 +5,7 @@ Require Import Sumbool.
 
 Require Export Kleene.
 Require Export Implementation.
+Require Import Arith.
 
 Module Export MC_Nat := Implementation.MC_Nat.
 
@@ -140,7 +141,6 @@ apply In_RecVarList; auto.
 Qed.
 
 Open Scope MC_scope.
-
 
 (** Choreography implementations are well-formed. *)
 Lemma Implementation_Main_WF : forall {n} (f:PRFunction n) ps q,
@@ -342,92 +342,193 @@ do 2 intro; case f; intros; simpl.
     rewrite plus_comm; auto with arith.
 Qed.
 
+Lemma all_pids_In : forall m n, m <= n -> List.In m (all_pids n).
+Proof.
+induction n; simpl; auto with arith.
+intro. inversion_clear H; auto.
+Qed.
+
+Lemma In_all_pids : forall m n, List.In m (all_pids n) -> m <= n.
+Proof.
+induction n; simpl; intros; inversion_clear H; auto; inversion H0; auto.
+Qed.
+
+Lemma all_pids_incl : forall m n, m <= n -> set_incl_Pid (all_pids m) (all_pids n).
+red; red; intros.
+apply all_pids_In. transitivity m; auto. apply In_all_pids; auto.
+Qed.
+
+Lemma MCC_pn_all_pids_incl : forall C m n, m <= n ->
+  (set_incl_Pid (MCC_pn C (fun _ => all_pids m)) (all_pids m))
+  -> (set_incl_Pid (MCC_pn C (fun _ => all_pids n)) (all_pids n)).
+Proof.
+induction C; simpl; unfold set_incl_Pid, set_incl; intros; auto.
+- inversion H1.
+- unfold set_incl_Pid, set_incl in IHC.
+  elim (set_union_elim _ _ _ _ H1); intros.
+  apply (all_pids_incl m); auto. apply H0. apply set_union_iff; auto.
+  apply IHC with m; auto. intros; apply H0. apply set_union_iff; auto.
+- unfold set_incl_Pid, set_incl in IHC.
+  elim (set_union_elim _ _ _ _ H1); intros.
+  apply (all_pids_incl m); auto. apply H0. apply set_union_iff; auto.
+  apply IHC with m; auto. intros; apply H0. apply set_union_iff; auto.
+- unfold set_incl_Pid, set_incl in IHC1, IHC2.
+  elim (set_union_elim _ _ _ _ H1); intros. elim (set_union_elim _ _ _ _ a); intros.
+  apply (all_pids_incl m); auto. apply H0. apply set_union_iff; left. apply set_union_iff; auto.
+  apply IHC1 with m; auto. intros; apply H0. apply set_union_iff; left. apply set_union_iff; auto.
+  apply IHC2 with m; auto. intros; apply H0. apply set_union_iff; auto.
+Qed.
+
 (*
-Lemma Zero_Procs_WF : forall d Hd ps q n X Y,
-  ~In q ps -> Choreography_WF (Implementation_aux Zero d Hd ps q n X Y).
+Lemma seq_compose_well_ann : forall {k m} (fs:t (PRFunction m) k) d Hd ps q i X Impl Y,
+  (forall p, In p ps -> p <= i) -> q + k <= i ->
+  (forall H p Hd' i' X' Y' n q', i <= i' -> q' + k <= i' -> List.In p (MCC_pn (Impl m fs[@H] Hd' ps q' (S i') X' Y') (fun _ => all_pids (i' + Pi fs[@H] + n))) -> p <= i' + Pi fs[@H] + n) ->
+ forall p,
+  List.In p (MCC_pn (seq_compose fs d Hd ps q (S i) X Impl Y) (fun _ => all_pids (i + vsum (map Pi fs)))) -> p <= i + vsum (map Pi fs).
 Proof.
-intros; induction d. inversion Hd.
-simpl. unfold Pack1; simpl.
-elim RecVar_dec; repeat split; simpl; auto.
-intro; apply H. eapply nth_In; eauto.
+induction k; intro.
++ refine (@case0 _ _ _ ); simpl; intros. inversion H2.
++ intro. revert k fs IHk. refine (@caseS _ _ _); intros.
+  revert H2; simpl. rewrite plus_assoc. elim Nat.ltb; intros.
+  - apply (H1 Fin.F1 p (Hd Fin.F1) i X Y _ q); auto with arith.
+    (* transitivity (q + S n); auto with arith. *)
+  - apply IHk with d (fun H => Hd (Fin.FS H)) ps (S q) (X+Gamma h) Impl Y; auto.
+    * intros; transitivity i; auto with arith.
+    * rewrite <- plus_n_Sm in H0; transitivity i; auto with arith.
+    * intros. apply (H1 (Fin.FS H3) _ Hd' i' X' Y' _ q'); auto.
+      transitivity (i + Pi h); auto with arith.
 Qed.
 
-Lemma Zero_Procs_initial : forall d Hd ps q n X Y,
-  initial (Implementation_aux Zero d Hd ps q n X Y).
+Lemma Implements_aux_well_ann : forall {m} (f:PRFunction m) d Hd ps q i X Y,
+  (forall p, In p ps -> p <= i) -> q <= i -> forall p,
+  List.In p (MCC_pn (Implementation_aux f d Hd ps q (S i) X Y) (fun _ => all_pids (i + Pi f))) -> p <= i + Pi f.
 Proof.
-intros; induction d. inversion Hd.
-simpl. unfold Pack1; simpl.
-elim RecVar_dec; simpl; auto.
-Qed.
+intros m f d; revert m f.
+induction d. inversion Hd.
+do 2 intro; case f; simpl; intros; revert H1.
+- unfold Pack1. rewrite plus_0_r.
+  elim RecVar_dec; simpl; intros. 2: inversion H1.
+  elim (set_union_elim _ _ _ _ H1); intros. inversion_clear a.
+  * apply H; eapply nth_In; eauto.
+  * revert H0. inversion_clear H2; inversion H0; auto.
+  * apply In_all_pids; auto.
+- unfold Pack1. rewrite plus_0_r.
+  elim RecVar_dec; simpl; intros. 2: inversion H1.
+  elim (set_union_elim _ _ _ _ H1); intros. inversion_clear a.
+  * apply H; eapply nth_In; eauto.
+  * revert H0. inversion_clear H2; inversion H0; auto.
+  * apply In_all_pids; auto.
+- unfold Pack1. rewrite plus_0_r.
+  elim RecVar_dec; simpl; intros. 2: inversion H1.
+  elim (set_union_elim _ _ _ _ H1); intros. inversion_clear a.
+  * apply H; eapply nth_In; eauto.
+  * revert H0. inversion_clear H2; inversion H0; auto.
+  * apply In_all_pids; auto.
+- set (Hd' := lt_S_n (Nat.max (depth g) (vmax (map depth fs))) d Hd).
+  set (Hfs := vmax_lt_map _ _ (max_lt_r _ _ _ Hd')).
+  set (Hg := max_lt_l _ _ _ Hd').
+  rename m into n; rename m0 into m.
+  elim Nat.ltb; intro.
+  * generalize (seq_compose_well_ann fs d Hfs ps (S i) (i+m) X (fun m f => Implementation_aux f d) Y); intros.
+    transitivity (S (i + m) + vsum (map Pi fs)). apply H2; auto.
+    + transitivity i; auto with arith.
+    + intros.
+      assert (forall p, In p ps -> p <= i'). transitivity i; auto. transitivity (S (i+m)); auto with arith.
+      assert (q' <= i'). transitivity (S i + m); auto.
+      generalize (IHd _ fs[@H3] Hd'0 ps q' i' X Y H7 H8).
+      intro.
+      apply In_all_pids. revert H6.
+      apply MCC_pn_all_pids_incl with (i' + Pi fs[@H3]); auto with arith.
+      red; red; intros. apply all_pids_In; eauto.
+    + 
 
-Lemma Zero_Procs_within_Xs : forall d Hd ps q n X Y Xs,
-  List.In X Xs -> List.In (S X) Xs ->
-  within_Xs Xs (Implementation_aux Zero d Hd ps q n X Y).
-Proof.
-intros; induction d. inversion Hd.
-simpl. unfold Pack1; simpl.
-elim RecVar_dec; simpl; auto.
-Qed.
+(* *)
 
-Lemma Succ_Procs_WF : forall d Hd ps q n X Y,
-  ~In q ps -> Choreography_WF (Implementation_aux Successor d Hd ps q n X Y).
-Proof.
-intros; induction d. inversion Hd.
-simpl. unfold Pack1; simpl.
-elim RecVar_dec; repeat split; simpl; auto.
-intro; apply H. eapply nth_In; eauto.
-Qed.
-
-Lemma Succ_Procs_initial : forall d Hd ps q n X Y,
-  initial (Implementation_aux Successor d Hd ps q n X Y).
-Proof.
-intros; induction d. inversion Hd.
-simpl. unfold Pack1; simpl.
-elim RecVar_dec; simpl; auto.
-Qed.
-
-Lemma Succ_Procs_within_Xs : forall d Hd ps q n X Y Xs,
-  List.In X Xs -> List.In (S X) Xs ->
-  within_Xs Xs (Implementation_aux Successor d Hd ps q n X Y).
-Proof.
-intros; induction d. inversion Hd.
-simpl. unfold Pack1; simpl.
-elim RecVar_dec; simpl; auto.
-Qed.
-
-Lemma Proj_Procs_WF : forall k m (Hp:k<m) d Hd ps q n X Y,
-  ~In q ps -> Choreography_WF (Implementation_aux (Projection Hp) d Hd ps q n X Y).
-Proof.
-intros; induction d. inversion Hd.
-simpl. unfold Pack1; simpl.
-elim RecVar_dec; repeat split; simpl; auto.
-intro; apply H. eapply nth_In; eauto.
-Qed.
-
-Lemma Proj_Procs_initial : forall k m (Hp:k<m) d Hd ps q n X Y,
-  initial (Implementation_aux (Projection Hp) d Hd ps q n X Y).
-Proof.
-intros; induction d. inversion Hd.
-simpl. unfold Pack1; simpl.
-elim RecVar_dec; simpl; auto.
-Qed.
-
-Lemma Proj_Procs_within_Xs : forall k m (Hp:k<m) d Hd ps q n X Y Xs,
-  List.In X Xs -> List.In (S X) Xs ->
-  within_Xs Xs (Implementation_aux (Projection Hp) d Hd ps q n X Y).
-Proof.
-intros; induction d. inversion Hd.
-simpl. unfold Pack1; simpl.
-elim RecVar_dec; simpl; auto.
-Qed.
-
-Lemma Recursion_Procs_WF : forall m (f:PRFunction m) g d Hd ps q n X Y,
-  ~In q ps -> Choreography_WF (Implementation_aux (Recursion f g) d Hd ps q n X Y).
-Proof.
-intros; induction d. inversion Hd.
-simpl. elim Nat.ltb.
-elim RecVar_dec; repeat split; simpl; auto.
-intro; apply H. eapply nth_In; eauto.
+- set (Hd' := lt_S_n (Nat.max (depth g) (depth h)) d Hd).
+  set (Hg := (max_lt_l _ _ _ Hd')).
+  set (Hh := (max_lt_r _ _ _ Hd')).
+  assert (forall p, In p (tl ps) -> p <= i+3).
+  1:{ intros. transitivity i; auto with arith. apply H, In_tail; auto. }
+  assert (S i <= i+3). rewrite plus_comm; simpl; auto.
+  generalize (IHd _ _ Hg (tl ps) (S i) (i+3) X Y H1 H2 p).
+  assert (forall p, In p (S (S i) :: S i :: tl ps) -> p <= i + 3 + Pi g).
+  1: {
+    intros. elim (In_elim H3); intros. rewrite <- H4, <- (plus_comm 3). auto with arith.
+    elim (In_elim H4); intros. rewrite <- H5, <- (plus_comm 3). simpl; auto with arith.
+    transitivity i; auto with arith. apply H, In_tail; auto.
+  }
+  assert (S (i + 2) <= i + 3 + Pi g). auto with arith.
+  generalize (IHd _ _ Hh (S (S i) :: S i :: tl ps) (S (i + 2)) (i+3+Pi g) (X+Gamma g+2) Y H3 H4 p).
+  do 2 intro.
+  assert (S (S i) <= i + (Pi g + Pi h + 3)) as Hi. transitivity (i+3); auto with arith. rewrite plus_comm; simpl; auto.
+  assert (S i <= i + (Pi g + Pi h + 3)) as Hi'. transitivity (i+3); auto with arith.
+  assert (S (i+2) <= i + (Pi g + Pi h + 3)) as Hi''. transitivity (i+3); auto with arith.
+  elim Nat.ltb. 2: elim RecVar_dec. 3: elim RecVar_dec. 4: elim RecVar_dec.
+  * intros.
+    apply In_all_pids. revert H7. apply MCC_pn_all_pids_incl with (i+3+Pi g).
+    rewrite <- plus_assoc, (plus_comm 3). auto with arith.
+    red; red; intros. apply all_pids_In; eauto.
+  * simpl; intros.
+    elim (set_union_elim _ _ _ _ H7); intro. inversion_clear a; inversion H8; auto.
+    + rewrite <- H9; auto.
+    + inversion H9.
+    + apply In_all_pids; auto.
+  * simpl; intros.
+    elim (set_union_elim _ _ _ _ H7); intro. inversion_clear a; inversion H8.
+    + transitivity i; auto with arith. eapply H, nth_In; auto.
+    + rewrite <- H9; auto.
+    + inversion H9.
+    + elim (set_union_elim _ _ _ _ b); intro. elim (set_union_elim _ _ _ _ a); intro.
+      ++ inversion_clear a0; inversion H8; auto.
+      ++ elim (set_union_elim _ _ _ _ b0); intro. inversion_clear a0.
+         rewrite <- H8; auto.
+         inversion_clear H8; inversion H9. rewrite <- H9. transitivity i; auto with arith.
+         apply In_all_pids; auto.
+      ++ apply In_all_pids; auto.
+  * simpl; intros.
+    elim (set_union_elim _ _ _ _ H7); intro. inversion_clear a; inversion H8; auto.
+    + rewrite <- H9; auto.
+    + inversion H9.
+    + elim (set_union_elim _ _ _ _ b); intro. inversion_clear a.
+      ++ rewrite <- H8; auto.
+      ++ inversion_clear H8; inversion H9; auto.
+      ++ elim (set_union_elim _ _ _ _ b0); intro. inversion_clear a.
+         rewrite <- H8; auto.
+         inversion_clear H8; inversion H9; auto.
+         apply In_all_pids; auto.
+  * rewrite (plus_comm (Pi g + Pi h)), plus_assoc, plus_assoc.
+    auto.
+- set (Hd' := lt_S_n (depth h) d Hd).
+  assert (forall p, In p (shiftin (S (i+1)) ps) -> p <= i+3).
+  1:{ intros. elim (shiftin_elim _ _ H1); auto with arith.
+      intro; rewrite <- H2, plus_comm, <- (plus_comm 3); simpl; auto. }
+  assert (S i <= i+3). rewrite plus_comm; simpl; auto.
+  generalize (IHd _ _ Hd' _ _ _ (X+1) Y H1 H2 p); intro.
+  assert (S (i+2) <= i + (Pi h + 3)) as Hi. rewrite <- (plus_comm 3); simpl; auto with arith.
+  assert (S i <= i + (Pi h + 3)) as Hi'. transitivity (S (i+2)); auto with arith.
+  assert (S (i+1) <= i + (Pi h + 3)) as Hi''. transitivity (S (i+2)); auto with arith.
+  elim RecVar_dec. 2: elim RecVar_dec.
+  * simpl; intro. elim (set_union_elim _ _ _ _ H4); intro. inversion_clear a; inversion H5; auto.
+    + rewrite <- H6; auto.
+    + inversion H6.
+    + apply In_all_pids; auto.
+  * simpl; intro. elim (set_union_elim _ _ _ _ H4); intro.
+    1: { inversion_clear a; inversion H5; auto; inversion H6; auto. }
+    elim (set_union_elim _ _ _ _ b); intro.
+    1: { inversion_clear a; inversion H5; auto; inversion H6; auto. }
+    elim (set_union_elim _ _ _ _ b0); intro.
+    1: { elim (set_union_elim _ _ _ _ a); intro.
+        inversion_clear a0; inversion H5; auto.
+        elim (set_union_elim _ _ _ _ b1); intro.
+        inversion_clear a0; inversion H5; auto; inversion H6; auto.
+        rewrite <- H6. transitivity i; auto with arith.
+        apply In_all_pids; auto. }
+    elim (set_union_elim _ _ _ _ b1); intro.
+    1: { inversion_clear a; inversion H5; auto; inversion H6; auto. }
+    elim (set_union_elim _ _ _ _ b2); intro.
+    1: { inversion_clear a; inversion H5; auto; inversion H6; auto. }
+    apply In_all_pids; auto.
+  * rewrite (plus_comm (Pi h)), plus_assoc; auto.
 Qed.
 *)
 
@@ -446,8 +547,14 @@ exists (RecVarList (0+Gamma f)); split.
   split. apply Implementation_aux_initial.
   split. apply Implementation_Procs_Vars_not_nil.
   apply Implementation_aux_within_Xs; simpl; auto.
-+ red.
-  unfold Vars; simpl.
++ red; intro. unfold Vars; simpl.
+  do 2 red; intros.
+  unfold Procs, Implementation, Procedures in H0.
+  admit.
+  (* apply Implements_aux_well_ann in H0.
+  - apply all_pids_In; auto.
+  - intros. apply Nat.max_le_iff. right; apply vmax_In; auto.
+  - apply Nat.le_max_l. *)
 Admitted.
 
 Lemma Implements'_WF : forall {n} (f:PRFunction n),
@@ -458,617 +565,87 @@ intro. elim (in_vec_k_to_n _ H); intros.
 inversion H0.
 Qed.
 
-Lemma Implementation_aux_converges : forall {n} (f:PRFunction n) d Hd ps q i X Defs ns y,
-  ~In q ps -> (forall p, In p ps -> p < i) -> q < i ->
-  (forall Y, X <= Y < X + Gamma f -> fst (Defs Y) <> List.nil) ->
-  (forall Y, X <= Y < X + Gamma f -> snd (Defs Y) = Implementation_aux f d Hd ps q i X Y) ->
-  converges f ns y -> 
-  forall (s:State), (forall H, s ps[@H] xx = ns[@H]) ->
-  exists s' tl, s' q xx = y /\ (forall p, p < i -> p <> q -> s' p xx = s p xx) /\
-  (Build_Program Defs (Call X),s) --[tl]-->* (Build_Program Defs (Call (X + Gamma f)),s').
+Lemma Implementation_aux_ge : forall {n} (f:PRFunction n) d Hd ps q i X Y,
+  Y >= X + Gamma f -> Implementation_aux f d Hd ps q i X Y = End.
 Proof.
 intros n f d; revert n f. induction d. inversion Hd.
-intros n f; case f; intros; rename H into Hqps, H0 into Hps, H1 into Hqn, H2 into HDefs, H3 into HDefs', H4 into Hf, H5 into Hinput.
-+ (* Zero *)
-  assert (X <= X < X + Gamma Zero). split; auto; rewrite plus_comm; auto with arith.
-  generalize (HDefs _ H), (HDefs' _ H).
-  simpl; unfold Pack1; simpl.
-  rewrite Rdec.eqb_refl. intros HX HX'.
-  elim (Call_reduce _ _ s HX); intros tl Htl.
-  rewrite HX' in Htl.
-  set (s' := update s q xx 0).
-  exists s', (tl ++ (L_Com ps[@Fin.F1] 0 q :: List.nil))%list.
-  rewrite (converges_Zero _ _ Hf).
-  split. apply update_read.
-  split. intros; apply update_read'. auto.
-  eapply MCT_Trans; eauto.
-  replace (L_Com ps[@Fin.F1] 0 q) with (forget (R_Com ps[@Fin.F1] 0 q xx)); auto.
-  econstructor; constructor. rewrite plus_comm; simpl. apply C_Com'.
-+ (* Successor *)
-  set (x := s ps[@Fin.F1] xx).
-  assert (X <= X < X + Gamma Zero). split; auto; rewrite plus_comm; auto with arith.
-  generalize (HDefs _ H), (HDefs' _ H).
-  simpl; unfold Pack1; simpl.
-  rewrite Rdec.eqb_refl. intros HX HX'.
-  elim (Call_reduce _ _ s HX); intros tl Htl.
-  rewrite HX' in Htl.
-  set (s' := update s q xx (S x)).
-  exists s', (tl ++ (L_Com ps[@Fin.F1] (S x) q :: List.nil))%list.
-  rewrite (converges_Successor _ _ Hf).
-  split. rewrite <- nth_hd, <- Hinput. apply update_read.
-  split. intros; apply update_read'. auto.
-  eapply MCT_Trans; eauto.
-  replace (L_Com ps[@Fin.F1] (S x) q) with (forget (R_Com ps[@Fin.F1] (S x) q xx)); auto.
-  econstructor; constructor. rewrite plus_comm; simpl. apply C_Com'.
-+ (* Projection *)
-  set (x := s ps[@Fin.of_nat_lt l] xx).
-  assert (X <= X < X + Gamma Zero). split; auto; rewrite plus_comm; auto with arith.
-  generalize (HDefs _ H), (HDefs' _ H).
-  simpl; unfold Pack1; simpl.
-  rewrite Rdec.eqb_refl. intros HX HX'.
-  elim (Call_reduce _ _ s HX); intros tl Htl.
-  rewrite HX' in Htl.
-  set (s' := update s q xx x).
-  exists s', (tl ++ (L_Com ps[@Fin.of_nat_lt l] x q :: List.nil))%list.
-  rewrite (converges_Projection _ _ _ _ _ Hf).
-  split. rewrite <- Hinput. apply update_read.
-  split. intros; apply update_read'. auto.
-  eapply MCT_Trans; eauto.
-  replace (L_Com ps[@Fin.of_nat_lt l] x q) with (forget (R_Com ps[@Fin.of_nat_lt l] x q xx)); auto.
-  econstructor; constructor. rewrite plus_comm; simpl. apply C_Com'.
-+ (* Composition *)
-  set (Hd' := lt_S_n (Nat.max (depth g) (vmax (map depth fs))) d Hd).
-  set (Hfs := vmax_lt_map _ _ (max_lt_r _ _ _ Hd')).
-  set (Hg := max_lt_l _ _ _ Hd').
-  elim (converges_Composition _ _ _ _ Hf); clear Hf; intros.
-  inversion_clear H. rename x into ms, H0 into H'fs, H1 into H'g.
-  (* Here we start directly with the loop *)
-  assert (exists sF tlF, (Build_Program Defs (Call X),s) --[tlF]-->* (Build_Program Defs (Call (X + vsum (map Gamma fs))),sF)
-    /\ (forall p, p<i -> sF p xx = s p xx)
-    /\ forall z H, converges (fs[@H]) ns z -> sF (seq_labels i fs)[@H] xx = z).
-  - assert (forall Y, X <= Y < X + vsum (map Gamma fs) -> X <= Y < X + Gamma (Composition g fs)).
-    1: {
-      intros. inversion_clear H; split; auto.
-      simpl. rewrite (plus_comm (Gamma g)).
-      etransitivity; eauto.
-      rewrite <- plus_0_r at 1. rewrite plus_assoc.
-      apply plus_lt_compat_l. apply Gamma_neq_zero.
-    }
-    generalize (fun Y HY => HDefs Y (H Y HY)).
-    clear HDefs; intro HDefs.
-    assert (exists k, forall Y, X <= Y < X + vsum (map Gamma fs) ->
-      snd (Defs Y) = seq_compose fs _ Hfs ps i (i+m+k) X (fun m f => Implementation_aux f d) Y).
-    1: { exists 0; intros. rewrite HDefs'; auto. rewrite Composition_Procs_fs, plus_0_r; auto. }
-    clearbody Hd' Hfs.
-    clear g H'g H Hd Hd' Hg HDefs'; rename H0 into HDefs'.
-    revert dependent X. revert dependent i. revert dependent s.
-    induction m.
-    * intros. exists s, List.nil.
-      rewrite <- (vector_0_inv fs). repeat split; auto.
-      simpl. rewrite plus_comm; constructor.
-      intros. inversion H.
-    * intros.
-      revert dependent ms. revert IHm.
-      revert dependent fs. revert m. refine (@caseS _ _ _); intros.
-      revert dependent t. revert IHm.
-      revert dependent ms. revert n0. refine (@caseS _ _ _); intros.
-      clear f. rename h into f, t0 into fs, h0 into x, t into xs, n0 into m.
-      (* First f... *)
-      assert (forall Y, X <= Y < X + Gamma f -> X <= Y < X + vsum (map Gamma (f::fs))).
-      1: { intros. inversion_clear H; split; auto. simpl. rewrite plus_assoc; auto with arith. }
-      elim HDefs'; clear HDefs'; intros k' HDefs'.
-      assert (i < i + S m + k').
-      1: { apply lt_le_trans with (i + S m); auto with arith. rewrite <- plus_n_Sm; auto with arith. }
-      elim IHd with k f (Hfs Fin.F1) ps i (i + S m + k') X Defs ns x s; auto.
-      2: { intro. apply (lt_irrefl i); auto. }
-      2: { transitivity i; auto. }
-      2: {
-        intros.
-        rewrite HDefs'; auto.
-        simpl. inversion_clear H1.
-        apply Nat.ltb_lt in H3; rewrite H3. auto.
-      }
-      2: { change (converges (hd (f::fs)) ns (hd (x::xs))). repeat rewrite <- nth_hd; auto. }
-      intros. destroy H1. rename x0 into sf, x1 into tlf.
-      (* ... then the rest. *)
-      elim IHm with fs (fun H => Hfs (Fin.FS H)) xs sf (S i) (X + Gamma f); intros.
-      2: { change (converges (tl (f::fs))[@H4] ns (tl (x::xs))[@H4]). rewrite <- nth_tl. apply H'fs. }
-      2: { assert (ps[@H4] < i). apply Hps; eapply nth_In; eauto.
-           rewrite H3; auto. transitivity i; auto. apply lt_neq; auto. }
-      2: { apply lt_le_trans with i; auto. }
-      2: { apply lt_le_trans with i; auto. }
-      2: {
-        apply HDefs. simpl. inversion_clear HY; split.
-        transitivity (X + Gamma f); auto with arith.
-        rewrite plus_assoc; auto.
-      }
-      2: {
-        exists (k' + Pi f); intros.
-        inversion_clear H4. rewrite <- plus_assoc in H6.
-        rewrite (HDefs' Y). 2: split; auto; transitivity (X + Gamma f); auto with arith.
-        simpl. generalize H5; intro.
-        apply le_not_lt, Nat.ltb_nlt in H5. rewrite H5.
-        replace (i + S m + k' + Pi f) with (S (i + m + (k' + Pi f))); auto.
-        repeat rewrite plus_assoc. rewrite <- plus_n_Sm; auto.
-      }
-      simpl (vsum (map Gamma (f::fs))).
-      destroy H4. rename x0 into s', x1 into tl'.
-      (* Wheee. *)
-      exists s', (tlf ++ tl')%list; repeat split; auto.
-      ++ rewrite plus_assoc. eapply MCT_Trans; eauto.
-      ++ intros; rewrite H6; auto.
-         apply H3. transitivity i; auto.
-         apply lt_neq; auto.
-      ++ intros. revert H8.
-         apply (hd_tl_induction' (fun x y => converges x ns z -> s' y xx = z)); auto.
-         simpl; intros. rewrite H6; auto. rewrite (converges_inj _ _ _ _ H8 (H'fs Fin.F1)); auto.
-  - destroy H. rename x into sF, x0 into tlF.
-    assert (X + Gamma (Composition g fs) = X + vsum (map Gamma fs) + Gamma g) as HX.
-    simpl. rewrite (plus_comm (Gamma g)), plus_assoc; auto.
-    elim IHd with m g Hg (seq_labels i fs) q (i+m) (X + vsum (map Gamma fs)) Defs ms y sF; auto.
-    * intros. destroy H2. rename x into s', x0 into tl'.
-      exists s', (tlF++tl')%list; repeat split; auto.
-      ++ intros. rewrite H4; auto. apply lt_le_trans with i; auto with arith.
-      ++ eapply MCT_Trans; eauto.
-         rewrite HX; auto.
-    * intro. elim (seq_labels_lt _ _ _ H2); intros.
-      elim (lt_irrefl q). apply lt_le_trans with i; auto.
-    * intros. elim (seq_labels_lt _ _ _ H2); auto.
-    * apply lt_le_trans with i; auto with arith.
-    * intros. inversion_clear H2. apply HDefs; split; auto.
-      transitivity (X + vsum (map Gamma fs)); auto with arith.
-      rewrite HX; auto.
-    * intros. inversion_clear H2. rewrite HDefs'.
-      rewrite Composition_Procs_g; auto. rewrite HX; auto.
-      split; auto. transitivity (X + vsum (map Gamma fs)); auto with arith.
-      rewrite HX; auto.
-+ (* Recursion *)
-  set (Hd' := lt_S_n (Nat.max (depth g) (depth h)) d Hd).
-  set (Hg := (max_lt_l _ _ _ Hd')).
-  set (Hh := (max_lt_r _ _ _ Hd')).
-  assert (forall H, ps[@H] < i) as Hpsi.
-  1: { intros. apply Hps. eapply nth_In; auto. }
-  (* Setting up for the base case, using the induction hypothesis on g *)
-  (* Call X,s -> Call (X + Gamma g),sg sg(ps) = s(ps), sg(init) = f(s(tl ps)) *)
-  assert (forall Y, X <= Y < X + Gamma g -> X <= Y < X + (Gamma g + Gamma h + 3)) as H'.
-  1: {
-    intros. inversion_clear H; split; simpl; auto.
-    transitivity (X + Gamma g); auto.
-    apply plus_lt_compat_l; auto with arith.
-    apply le_lt_trans with (Gamma g + Gamma h); auto with arith.
-    rewrite <- (plus_comm 3); simpl; auto.
-  }
-  assert (forall Y, X <= Y < X + Gamma g -> fst (Defs Y) <> List.nil) as HgDefs. eauto.
-  assert (forall Y, X <= Y < X + Gamma g -> snd (Defs Y) = Implementation_aux g _ Hg (tl ps) i (i+3) X Y) as HgDefs'.
-  1: {
-    intros. elim H; intros. generalize (HDefs' _ (H' _ H)).
-    rewrite Recursion_Procs_g; auto.
-  }
-  assert (~In i (tl ps)) as Hi.
-  1: { intro. apply (lt_irrefl i). apply Hps. apply In_tail; auto. }
-  assert (i < i+3) as Hi'. rewrite plus_comm; simpl; auto.
-  assert (forall p, In p (tl ps) -> p < i+3) as Hpsg.
-  1: { intros. transitivity i; auto. apply Hps, In_tail; auto. }
-  elim (converges_Recursion_full _ _ _ _ Hf 0); auto with arith.
-  intros g0 Hg0.
-  assert (forall H, s (tl ps)[@H] xx = (tl ns)[@H]) as Hinput'.
-  1: intro; repeat rewrite <- nth_tl; auto.
-  elim (IHd _ _ Hg (tl ps) i (i+3) _ _ (tl ns) _ Hi Hpsg Hi' HgDefs HgDefs' Hg0 s Hinput'); intros.
-  destroy H.
-  rename x into sg, x0 into tlg, H0 into Hsg, H1 into Hsg', H into Htlg.
-  clear Hi HgDefs HgDefs' H' Hpsg Hg.
-  (* Call X + Gamma g,sg -> Call (X + Gamma g + 1),s' s'(ps) = s(ps), s'(S init) = 0, s'(init) = f(s(tl ps)) *)
-  assert (X <= X + Gamma g < X + Gamma (Recursion g h)).
-  1: {
-    split; auto with arith.
-    apply plus_lt_compat_l. simpl. rewrite <- (plus_comm 3).
-    transitivity (2 + Gamma g); simpl; auto with arith.
-  }
-  elim (Call_reduce Defs (X + Gamma g) sg); auto. intros.
-  rename x into tlg'.
-  rewrite HDefs', Recursion_Procs_0 in H0; auto.
-  generalize (C_Com' Defs (i+2) zero (S i) xx (Call (X + Gamma g + 1)) sg); intro.
-  simpl in H1. generalize (MCP_To_intro _ _ _ _ _ _ H1).
-  clear H1; simpl; intro.
-  set (P := Build_Program Defs (Call (X + Gamma g + 1))).
-  generalize (MCT_Trans _ _ _ _ _ Htlg (MCT_Trans _ _ _ _ _ H0 (MCT_Step _ _ _ _ _ H1 (MCT_Refl _)))).
-  clear H0 H1; fold P; intro HP.
-  set (t := (tlg ++ tlg' ++ L_Com (i+2) 0 (S i) :: List.nil)%list).
-  set (s0 := update sg (S i) xx 0).
-  fold t s0 in HP.
-  assert (s0 i xx = g0) as Hs0i. rewrite <- Hsg. apply update_read'; auto.
-  assert (s0 (S i) xx = 0) as Hs0Si. apply update_read.
-  assert (forall H, s0 ps[@H] xx = ns[@H]) as Hs0.
-  1: {
-    intros. rewrite <- Hinput, <- Hsg'; auto.
-    apply update_read'; auto.
-    apply gt_neq; red; transitivity i; auto.
-    transitivity i; auto.
-    apply lt_neq; auto.
-  }
-  assert (forall p, p < i -> s0 p xx = s p xx) as Hs0'.
-  1: {
-    intros; unfold s0; rewrite update_read'.
-    apply Hsg'; auto with arith. apply lt_neq; auto.
-    apply gt_neq; red; transitivity i; auto.
-  }
-  clearbody t s0. clear sg Hsg Hsg' Htlg.
-  (* Loop invariant *)
-  assert (forall m, m <= hd ns -> exists t' s' y', (P,s0) --[ t' ]-->* (P,s')
-    /\ converges (Recursion g h) (m::tl ns) y' /\ s' i xx = y' /\ s' (S i) xx = m /\ forall j, j < i -> s' j xx = s0 j xx).
-  - induction m; intros.
-    * exists List.nil, s0, g0; repeat split; auto. constructor.
-    * elim IHm; auto with arith; clear IHm.
-      intros tlI H'; destroy H'.
-      rename x into sI, x0 into yI, H1 into HI.
-      assert (X <= X + Gamma g + 1 < X + Gamma (Recursion g h)).
-      1: { split; simpl; auto with arith.  repeat (rewrite <- plus_assoc; apply plus_lt_compat_l); auto with arith. }
-      elim (Call_reduce Defs (X + Gamma g + 1) sI); intros; auto.
-      rename x into tlU, H5 into HU.
-      rewrite HDefs', Recursion_Procs_1 in HU; auto.
-      unfold IfEq in HU.
-      generalize (MCP_To_intro _ _ _ _ _ _ (C_Com' Defs ps[@Fin.F1] this (S i) yy (If (S i) ? compare Then Send i this q;; Call (X + Gamma g + Gamma h + 3) Else Call (X + Gamma g + 2)) sI)).
-      simpl; intro.
-      assert (beval_on_state compare (update sI (S i) yy (sI ps[@Fin.F1] xx)) (S i) = false).
-      1: { 
-        unfold beval_on_state, beval, MC_BEval.eval.
-        rewrite update_read. rewrite update_read''. 2: discriminate.
-        rewrite H4. rewrite H'; auto. rewrite Hs0.
-        rewrite Nat.eqb_neq. apply lt_neq.
-        rewrite nth_hd; auto.
-      }
-      generalize (MCP_To_intro _ _ _ _ _ _ (C_Else' Defs (S i) compare (Send i this q;; Call (X + Gamma g + Gamma h + 3)) (Call (X + Gamma g + 2)) _ H6)).
-      simpl; clear H6; intro.
-      assert (X <= X + Gamma g + 2 < X + Gamma (Recursion g h)).
-      1: { split; simpl; auto with arith.  repeat (rewrite <- plus_assoc; apply plus_lt_compat_l); auto with arith. }
-      set (sU := update sI (S i) yy (sI ps[@Fin.F1] xx)).
-      generalize (MCT_Trans _ _ _ _ _ HU (MCT_Step _ _ _ _ _ H5 (MCT_Step _ _ _ _ _ H6 (MCT_Refl _)))).
-      clear HU H5 H6; intro.
-      (* Setting up for the induction hypothesis on h *)
-      assert (i+2 < i+3+Pi g) as Hi''; intros. auto with arith.
-      assert (forall p, In p (S i::i::tl ps) -> p < i+3+Pi g) as Hpsh; intros.
-      1: { elim (In_elim H6); intro.
-        rewrite <- H8. rewrite <- plus_assoc. rewrite plus_comm; simpl.
-        rewrite plus_comm; auto with arith.
-        elim (In_elim H8); intro.
-        rewrite H9; apply le_lt_trans with (p+0); auto with arith.
-        transitivity i. apply Hps, In_tail; auto.
-        apply le_lt_trans with (i+0); auto with arith.
-      }
-      assert (~In (i+2) (S i::i::tl ps)) as Hi; intros.
-      1: { intro. elim (In_elim H6).
-        apply lt_neq. rewrite plus_comm; auto.
-        intro; elim (In_elim H8).
-        apply lt_neq; rewrite plus_comm; simpl; auto.
-        intro. apply (lt_irrefl i).
-        transitivity (i+2). rewrite plus_comm; simpl; auto.
-        apply Hps, In_tail; auto.
-      }
-      assert (forall Y, X + Gamma g + 2 <= Y < X + Gamma g + 2 + Gamma h -> X <= Y < X + (Gamma g + Gamma h + 3)) as H''.
-      1: {
-        intros. inversion_clear H6; split; simpl.
-        transitivity (X + Gamma g + 2); auto with arith.
-        repeat rewrite <- plus_assoc.
-        repeat rewrite <- plus_assoc in H9.
-        rewrite (plus_comm 2) in H9.
-        etransitivity; eauto.
-        repeat apply plus_lt_compat_l; auto with arith.
-      }
-      assert (forall Y, X + Gamma g + 2 <= Y < X + Gamma g + 2 + Gamma h -> fst (Defs Y) <> List.nil) as HhDefs; auto.
-      assert (forall Y, X + Gamma g + 2 <= Y < X + Gamma g + 2 + Gamma h -> snd (Defs Y) = Implementation_aux h d Hh (S i :: i :: tl ps) (i + 2) (i + 3 + Pi g) (X + Gamma g + 2) Y) as HhDefs'; auto.
-      1: {
-        intros. unfold Hh, Hd'; rewrite <- Recursion_Procs_h with (q:=q); auto.
-        replace (X + Gamma g + Gamma h + 2) with (X + Gamma g + 2 + Gamma h); auto.
-        repeat rewrite <- plus_assoc. rewrite (plus_comm 2); auto.
-      }
-      assert (forall H, sU (S i::i::tl ps)[@H] xx = (m::yI::tl ns)[@H]) as Hinput''; intros.
-      1: {
-        replace (sU (S i::i::tl ps)[@H6] xx) with (map (fun y => sU y xx) (S i::i::tl ps))[@H6].
-        2: rewrite (nth_map _ _ _ _ (eq_refl _)); auto.
-        apply hd_tl_eq. 2: apply hd_tl_eq.
-        * simpl. unfold sU; rewrite update_read''; auto. discriminate.
-        * simpl. unfold sU; rewrite update_read'; auto.
-        * simpl. intros. rewrite (nth_map _ _ _ _ (eq_refl _)).
-          unfold sU; rewrite update_read'; auto.
-          repeat rewrite <- nth_tl. rewrite <- Hs0; auto.
-          apply gt_neq; red.
-          transitivity i; auto. rewrite <- nth_tl; auto.
-      }
-      elim (converges_Recursion_full _ _ _ _ Hf (S m)); auto; intros.
-      elim (converges_Recursion_step _ _ _ m _ H6); simpl; auto. intros.
-      inversion_clear H8.
-      rewrite (converges_inj _ _ _ _ H9 H2) in H10; clear x0 H9.
-      elim (IHd _ _ Hh _ _ _ _ _ _ _ Hi Hpsh Hi'' HhDefs HhDefs' H10 _ Hinput''); intros.
-      rename x0 into sF; destroy H8.
-      rename x0 into tlF.
-      (* After calling h *)
-      repeat rewrite <- plus_assoc in H8; rewrite (plus_comm 2) in H8.
-      repeat rewrite plus_assoc in H8.
-      assert (X <= X + Gamma g + Gamma h + 2 < X + (Gamma g + Gamma h + 3)).
-      1: { split; auto with arith.
-        repeat rewrite <- plus_assoc; repeat apply plus_lt_compat_l; auto.
-      }
-      elim (Call_reduce Defs (X + Gamma g + Gamma h + 2) sF); auto; intros.
-      rewrite HDefs', Recursion_Procs_2 in H13; auto.
-      generalize (MCP_To_intro _ _ _ _ _ _ (C_Com' Defs (i+2) this i xx (Send (S i) this (i+2);; Send (i+2) succ_this (S i);; Call (X + Gamma g + 1)) sF)).
-      simpl. set (sF' := update sF i xx (sF (i+2) xx)); intros.
-      generalize (MCP_To_intro _ _ _ _ _ _ (C_Com' Defs (S i) this (i+2) xx (Send (i+2) succ_this (S i);; Call (X + Gamma g + 1)) sF')).
-      simpl. set (sF'' := update sF' (i+2) xx (sF' (S i) xx)); intros.
-      generalize (MCP_To_intro _ _ _ _ _ _ (C_Com' Defs (i+2) succ_this (S i) xx (Call (X + Gamma g + 1)) sF'')).
-      simpl. set (sF''' := update sF'' (S i) xx (S (sF'' (i+2) xx))); intros.
-      exists (tlI ++ (tlU ++ L_Com ps[@Fin.F1] (sI ps[@Fin.F1] xx) (S i) :: L_Tau (S i) :: List.nil) ++ tlF ++ x0 ++ L_Com (i+2) (sF (i+2) xx) i :: L_Com (S i) (sF' (S i) xx) (i+2) :: L_Com (i+2) (S (sF'' (i+2) xx)) (S i) :: List.nil)%list.
-      exists sF''', x. repeat split; auto.
-      ++ do 4 (eapply MCT_Trans; eauto).
-         do 3 (eapply MCT_Step; eauto).
-         constructor.
-      ++ unfold sF''', sF'', sF'.
-         do 2 (rewrite update_read'; auto).
-         rewrite update_read; auto.
-         apply gt_neq; rewrite plus_comm; simpl; auto.
-      ++ unfold sF''', sF'', sF'.
-         rewrite update_read.
-         rewrite update_read.
-         rewrite update_read'; auto.
-         rewrite H11; auto.
-         2: {
-           rewrite <- plus_assoc; rewrite (plus_comm 3).
-           rewrite plus_assoc; rewrite plus_comm.
-           simpl; auto with arith.
-         }
-         2: { apply lt_neq; rewrite plus_comm; auto. }
-         unfold sU. rewrite update_read''; auto. discriminate.
-      ++ unfold sF''', sF'', sF'; intros.
-         rewrite update_read.
-         repeat rewrite update_read'.
-         rewrite H11; auto with arith.
-         unfold sU. rewrite update_read'; auto.
-         apply gt_neq; red; transitivity i; auto.
-         apply lt_neq; red; transitivity i; auto with arith.
-         apply gt_neq; auto.
-         apply gt_neq; red; transitivity i; auto. rewrite plus_comm; simpl; auto.
-         apply gt_neq; red; transitivity i; auto with arith.
-  - elim (H0 _ (le_refl _)); clear H0; intros tl Htl.
-    destroy Htl.
-    rename x into sF.
-    rewrite <- eta in H1.
-    rewrite <- (converges_inj _ _ _ _ Hf H1) in H2; clear H1 x0.
-    assert (X <= X + Gamma g + 1 < X + Gamma (Recursion g h)).
-    1: {
-      split; auto with arith.
-      simpl. repeat rewrite <- plus_assoc; repeat apply plus_lt_compat_l.
-      rewrite plus_comm; auto with arith.
-    }
-    elim (Call_reduce Defs (X + Gamma g + 1) sF); auto; intros.
-    rewrite HDefs', Recursion_Procs_1 in H4; auto.
-    rename x into tlU, H4 into HU.
-    unfold IfEq in HU.
-    generalize (MCP_To_intro _ _ _ _ _ _ (C_Com' Defs ps[@Fin.F1] this (S i) yy (If (S i) ? compare Then Send i this q;; Call (X + Gamma g + Gamma h + 3) Else Call (X + Gamma g + 2)) sF)).
-    simpl; intro.
-    assert (beval_on_state compare (update sF (S i) yy (sF ps[@Fin.F1] xx)) (S i) = true).
-    1: { 
-      unfold beval_on_state, beval, MC_BEval.eval.
-      rewrite update_read. rewrite update_read''. 2: discriminate.
-      rewrite H3. rewrite Htl; auto. rewrite Hs0.
-        rewrite Nat.eqb_eq. rewrite nth_hd; auto.
-    }
-    generalize (MCP_To_intro _ _ _ _ _ _ (C_Then' Defs (S i) compare (Send i this q;; Call (X + Gamma g + Gamma h + 3)) (Call (X + Gamma g + 2)) _ H5)).
-    set (sF' := update sF (S i) yy (sF ps[@Fin.F1] xx)).
-    simpl; clear H5; intro.
-    generalize (MCP_To_intro _ _ _ _ _ _ (C_Com' Defs i this q xx (Call (X + Gamma g + Gamma h + 3)) sF')).
-    simpl; set (sF'' := update sF' q xx (sF' i xx)); intro.
-    exists sF'', (t ++ tl ++ (tlU ++ L_Com ps[@Fin.F1] (sF ps[@Fin.F1] xx) (S i) :: L_Tau (S i) :: L_Com i (sF' i xx) q :: List.nil))%list.
-    repeat split; auto.
-    * unfold sF'', sF'. rewrite update_read.
-      rewrite update_read'; auto.
-    * unfold sF'', sF'. intros; repeat rewrite update_read'; auto.
-      2: apply gt_neq; red; transitivity i; auto.
-      rewrite Htl; auto.
-    * do 3 (eapply MCT_Trans; eauto).
-      do 3 (eapply MCT_Step; eauto).
-      do 2 rewrite <- (plus_assoc X). constructor.
-+ (* Minimization *)
-  set (Hd' := lt_S_n (depth h) d Hd).
-  assert (forall H, ps[@H] < i) as Hpsi.
-  1: { intros. apply Hps. eapply nth_In; auto. }
-  assert (S X = X + 1) as HXSX. rewrite plus_comm; auto.
-  (* Initialization *)
-  assert (X <= X < X + Gamma (Minimization h)).
-  1: {
-    split; auto with arith.
-    apply le_lt_trans with (X + 0); auto with arith.
-    apply plus_lt_compat_l; apply Gamma_neq_zero.
-  }
-  elim (Call_reduce Defs X s); auto. intros tl0 H00.
-  rewrite HDefs' in H00; auto.
-  rewrite Minimization_Procs_0 in H00.
-  generalize (MCP_To_intro _ _ _ _ _ _ (C_Com' Defs (i+2) zero (i+1) xx (Call (X+1)) s)).
-  simpl. set (s0 := update s (i+1) xx 0); intro.
-  (* Setting up for the induction hypothesis on h *)
-  assert (forall Y, X + 1 <= Y < X + 1 + Gamma h -> X <= Y < X + (Gamma h + 2)) as H'.
-  1: {
-    intros. inversion_clear H1; split; simpl.
-    transitivity (X + 1); auto with arith.
-    transitivity (X + 1 + Gamma h); auto.
-    rewrite <- (plus_comm 2), plus_assoc.
-    auto with arith.
-  }
-  assert (forall Y, X + 1 <= Y < X + 1 + Gamma h -> fst (Defs Y) <> List.nil) as HhDefs. eauto.
-  assert (forall Y, X + 1 <= Y < X + 1 + Gamma h -> snd (Defs Y) = Implementation_aux h _ Hd' (shiftin (i+1) ps) i (i+3) (X+1) Y) as HhDefs'.
-  1: {
-    intros. elim H1; intros. generalize (HDefs' _ (H' _ H1)).
-    rewrite Minimization_Procs_h; auto.
-    split; auto.
-    rewrite <- plus_assoc, <- (plus_comm 1), plus_assoc; auto.
-  }
-  assert (~In i (shiftin (i+1) ps)) as Hi.
-  1: {
-    intro. apply (lt_irrefl i). elim (shiftin_elim _ _ H1); auto.
-    intros; rewrite <- H2 at 2; auto. rewrite plus_comm; auto.
-  }
-  assert (i < i+3) as Hi'. rewrite plus_comm; simpl; auto.
-  assert (forall p, In p (shiftin (i+1) ps) -> p < i+3) as Hpsh.
-  1: {
-    intros. elim (shiftin_elim _ _ H1); auto.
-    intro. rewrite <- H2; simpl; auto with arith.
-    transitivity i; auto.
-  }
-  assert (exists z, converges h (shiftin 0 ns) z).
-  1: {
-    elim (eq_nat_dec y 0); intros.
-    + exists 0. apply converges_Minimization.
-      rewrite <- a; auto.
-    + elim (converges_Minimization_mon _ _ _ Hf) with 0; eauto.
-      apply neq_0_lt; auto.
-  }
-  inversion_clear H1.
-  assert (forall H, s0 (shiftin (i+1) ps)[@H] xx = (shiftin 0 ns)[@H]) as Hinput'.
-  1: {
-    intro.
-    replace (s0 (shiftin (i+1) ps)[@H1] xx) with (map (fun y => s0 y xx) (shiftin (i+1) ps))[@H1]; auto.
-    2: rewrite (nth_map _ _ _ _ (eq_refl _)); auto.
-    rewrite map_shiftin.
-    apply shiftin_eq.
-    unfold s0. rewrite plus_comm; apply update_read.
-    intro. rewrite nth_map'. unfold s0; rewrite update_read'; auto.
-    apply gt_neq; red. transitivity i; auto. rewrite plus_comm; auto.
-  }
-  elim (IHd _ _ Hd' _ _ _ _ _ _ _ Hi Hpsh Hi' HhDefs HhDefs' H2 _ Hinput'); intros.
-  rename x0 into sI; destroy H1.
-  rename x0 into tlI, H1 into HI.
-  replace (X + 1 + Gamma h) with (X + Gamma h + 1) in HI.
-  2: repeat rewrite <- plus_assoc; rewrite <- (plus_comm 1); auto.
-  generalize (MCT_Trans _ _ _ _ _ H00 (MCT_Step _ _ _ _ _ H0 HI)).
-  set (P := Build_Program Defs (Call (X + Gamma h + 1))).
-  clear H0 H00 HI; intro HI.
-  assert (X <= X + Gamma h + 1 < X + Gamma (Minimization h)).
-  1: { split; simpl; auto with arith. rewrite plus_assoc; auto with arith. }
-  (* Loop *)
-  assert (forall m, m <= y -> exists t' s' y', (P,sI) --[ t' ]-->* (P,s')
-    /\ converges h (shiftin m ns) y' /\ s' i xx = y' /\ s' (i+1) xx = m /\ forall j, j < i -> s' j xx = s0 j xx).
-  - induction m; intros.
-    * exists List.nil, sI, x; repeat split; auto. constructor.
-      rewrite H4; auto with arith. unfold s0. rewrite plus_comm, update_read; auto.
-      apply gt_neq. red; rewrite plus_comm; auto.
-      intros; apply H4. transitivity i; auto. apply lt_neq; auto.
-    * elim IHm; auto with arith; clear IHm.
-      intros tlI' H''; destroy H''.
-      rename x1 into yI, x0 into sI', H5 into HI'.
-      elim (Call_reduce Defs (X + Gamma h + 1) sI'); intros; auto.
-      rename x0 into tlU, H5 into HU.
-      rewrite HDefs', Minimization_Procs_1 in HU; auto.
-      generalize (MCP_To_intro _ _ _ _ _ _ (C_Com' Defs (i+1) zero (i+2) xx (IfEq (i+2) i (Send (i+1) this q;; Call (X + Gamma h + 2)) (Send (i+1) this (i+2);; Send (i+2) succ_this (i+1);; Call (X+1))) sI')).
-      simpl. set (s1 := update sI' (i+2) xx 0); intro.
-      generalize (MCP_To_intro _ _ _ _ _ _ (C_Com' Defs i this (i+2) yy (Cond (i+2) compare (Send (i+1) this q;; Call (X + Gamma h + 2)) (Send (i+1) this (i+2);; Send (i+2) succ_this (i+1);; Call (X+1))) s1)).
-      simpl. set (s2 := update s1 (i+2) yy (s1 i xx)); intro.
-      assert (beval_on_state compare s2 (i+2) = false).
-      1: {
-        unfold beval_on_state, beval, MC_BEval.eval.
-        apply Nat.eqb_neq.
-        unfold s2, s1.
-        rewrite update_read, update_read''; auto. 2: discriminate.
-        rewrite update_read, update_read'.
-        rewrite H7.
-        elim (converges_Minimization_mon _ _ _ Hf m); auto.
-        intros. rewrite (converges_inj _ _ _ _ H6 H10); discriminate.
-        apply gt_neq; rewrite plus_comm; simpl; auto.
-      }
-      generalize (MCP_To_intro _ _ _ _ _ _ (C_Else' Defs _ _ (Send (i+1) this q;; Call (X+Gamma h+2)) (Send (i+1) this (i+2);; Send (i+2) succ_this (i+1);; Call (X+1)) _ H10)).
-      simpl; clear H10; intro.
-      generalize (MCP_To_intro _ _ _ _ _ _ (C_Com' Defs (i+1) this (i+2) xx (Send (i+2) succ_this (i+1);; Call (X+1)) s2)).
-      simpl. set (s3 := update s2 (i+2) xx (s2 (i+1) xx)); intro.
-      generalize (MCP_To_intro _ _ _ _ _ _ (C_Com' Defs (i+2) succ_this (i+1) xx (Call (X+1)) s3)).
-      simpl. set (s4 := update s3 (i+1) xx (S (s3 (i+2) xx))); intro.
-      (* IH on H again *)
-      assert (exists z, converges h (shiftin (S m) ns) z).
-      1: {
-        inversion H1; intros.
-        + rewrite H13. elim (converges_Minimization _ _ _ Hf); intros.
-          exists 0, x0; eauto.
-        + elim (converges_Minimization_mon _ _ _ Hf) with (S m); eauto.
-          rewrite <- H14; auto with arith.
-      }
-      inversion_clear H13. rename x0 into x'.
-      assert (forall H, s4 (shiftin (i+1) ps)[@H] xx = (shiftin (S m) ns)[@H]) as Hinput''.
-      1: {
-        intro.
-        replace (s4 (shiftin (i+1) ps)[@H13] xx) with (map (fun y => s4 y xx) (shiftin (i+1) ps))[@H13]; auto.
-        2: rewrite (nth_map _ _ _ _ (eq_refl _)); auto.
-        rewrite map_shiftin.
-        apply shiftin_eq.
-        + unfold s4, s3, s2, s1.
-          repeat rewrite update_read. repeat rewrite update_read'.
-          2: apply gt_neq; red; auto with arith.
-          2: apply gt_neq; red; auto with arith.
-          rewrite <- H8; auto.
-        + intro. rewrite nth_map'. unfold s4, s3, s2, s1.
-          assert (i+2<>ps[@H15]). apply gt_neq; red; transitivity i; auto. rewrite plus_comm; simpl; auto.
-          repeat rewrite update_read'; auto.
-          2: apply gt_neq; red; auto with arith.
-          rewrite H'', <- Hinput; auto.
-          unfold s0. apply update_read'; auto.
-          apply gt_neq; red; rewrite plus_comm. transitivity i; auto.
-      }
-      elim (IHd _ _ Hd' _ _ _ _ _ _ _ Hi Hpsh Hi' HhDefs HhDefs' H14 _ Hinput''); intros.
-      rename x0 into sL; destroy H13.
-      rename x0 into tlL, H13 into HL.
-      replace (X + 1 + Gamma h) with (X + Gamma h + 1) in HL.
-      2: repeat rewrite <- plus_assoc; rewrite <- (plus_comm 1); auto.
-      fold P in HL, HU.
-      eexists; exists sL, x'; repeat split; auto.
-      -- do 2 (eapply MCT_Trans; eauto).
-         do 5 (eapply MCT_Step; eauto).
-      -- rewrite H16; auto with arith. 2: rewrite plus_comm; simpl; auto.
-         unfold s4, s3, s2, s1.
-         do 2 rewrite update_read. repeat rewrite update_read'.
-         2: apply gt_neq; red; auto with arith.
-         2: apply gt_neq; red; auto with arith.
-         rewrite <- H8; auto.
-      -- intros. rewrite H16. 2: transitivity i; auto with arith. 2: apply lt_neq; auto.
-         assert (i+2 <> j). apply gt_neq; red; rewrite plus_comm. transitivity i; simpl; auto.
-         unfold s4, s3, s2, s1. rewrite <- (plus_comm 1).
-         rewrite update_read. repeat rewrite update_read'; auto.
-         apply gt_neq; red; transitivity i; auto.
-  - elim (H1 y); auto.
-    intros tlL HL; destroy HL.
-    rename x0 into sL.
-    rewrite (converges_inj _ _ _ _ H6 (converges_Minimization _ _ _ Hf)) in H7; clear x1 H6.
-    elim (Call_reduce Defs (X + Gamma h + 1) sL); intros; auto.
-    rename x0 into tlU, H6 into HU.
-    rewrite HDefs', Minimization_Procs_1 in HU; auto.
-    generalize (MCP_To_intro _ _ _ _ _ _ (C_Com' Defs (i+1) zero (i+2) xx (IfEq (i+2) i (Send (i+1) this q;; Call (X + Gamma h + 2)) (Send (i+1) this (i+2);; Send (i+2) succ_this (i+1);; Call (X+1))) sL)).
-    simpl. set (s1 := update sL (i+2) xx 0); intro.
-    generalize (MCP_To_intro _ _ _ _ _ _ (C_Com' Defs i this (i+2) yy (Cond (i+2) compare (Send (i+1) this q;; Call (X + Gamma h + 2)) (Send (i+1) this (i+2);; Send (i+2) succ_this (i+1);; Call (X+1))) s1)).
-    simpl. set (s2 := update s1 (i+2) yy (s1 i xx)); intro.
-    assert (beval_on_state compare s2 (i+2) = true).
-    1: {
-      unfold beval_on_state, beval, MC_BEval.eval.
-      apply Nat.eqb_eq.
-      unfold s2, s1.
-      rewrite update_read, update_read''; auto. 2: discriminate.
-      rewrite update_read, update_read'; auto.
-      apply gt_neq; rewrite plus_comm; simpl; auto.
-    }
-    generalize (MCP_To_intro _ _ _ _ _ _ (C_Then' Defs _ _ (Send (i+1) this q;; Call (X+Gamma h+2)) (Send (i+1) this (i+2);; Send (i+2) succ_this (i+1);; Call (X+1)) _ H10)).
-    simpl; clear H10; intro.
-    generalize (MCP_To_intro _ _ _ _ _ _ (C_Com' Defs (i+1) this q xx (Call (X+Gamma h+2)) s2)).
-    simpl. set (s3 := update s2 q xx (s2 (i+1) xx)); intro.
-    exists s3; eexists. repeat split; auto.
-    * unfold s3, s2, s1.
-      rewrite update_read.
-      rewrite update_read'. 2: apply gt_neq; auto with arith.
-      rewrite update_read'; auto. apply gt_neq; auto with arith.
-    * intros. unfold s3, s2, s1.
-      rewrite update_read'; auto.
-      rewrite update_read'. 2: apply gt_neq; auto with arith.
-      rewrite update_read'. 2: apply gt_neq; auto with arith.
-      rewrite HL; auto.
-      unfold s0. apply update_read'. apply gt_neq; auto with arith.
-    * do 3 (eapply MCT_Trans; eauto).
-      do 4 (eapply MCT_Step; eauto).
-      rewrite plus_assoc; constructor.
+intros n f. case f; intros.
++ simpl in H; red in H. rewrite plus_comm in H.
+  simpl. unfold Pack1, RecVar_dec; simpl.
+  assert (Y <> X). apply gt_neq; auto with arith.
+  rewrite <- Rdec.eqb_neq in H0. rewrite H0; auto.
++ simpl in H; red in H. rewrite plus_comm in H.
+  simpl. unfold Pack1, RecVar_dec; simpl.
+  assert (Y <> X). apply gt_neq; auto with arith.
+  rewrite <- Rdec.eqb_neq in H0. rewrite H0; auto.
++ simpl in H; red in H. rewrite plus_comm in H.
+  simpl. unfold Pack1, RecVar_dec; simpl.
+  assert (Y <> X). apply gt_neq; auto with arith.
+  rewrite <- Rdec.eqb_neq in H0. rewrite H0; auto.
++ red in H.
+  simpl.
+  assert (Y >= X + vsum (map Gamma fs)). red. transitivity (X + (Gamma (Composition g fs))); simpl; auto with arith.
+  apply le_not_lt in H0. rewrite <- Nat.ltb_nlt in H0. rewrite H0.
+  apply IHd; rewrite <- plus_assoc, <- (plus_comm (Gamma g)); auto.
++ red in H.
+  simpl; unfold RecVar_dec.
+  assert (Y > X + Gamma g + 1).
+  1: { red. apply lt_le_trans with (X + (Gamma (Recursion g h))); simpl; auto.
+       repeat (rewrite <- plus_assoc; apply plus_lt_compat_l). rewrite plus_comm. simpl; auto with arith. }
+  assert (Y >= X + Gamma g). red; red in H0. transitivity (X + Gamma g + 1); auto with arith.
+  apply le_not_lt in H1. rewrite <- Nat.ltb_nlt in H1. rewrite H1.
+  assert (Y <> X + Gamma g). apply gt_neq; auto. red. transitivity (X + Gamma g + 1); auto. rewrite <- (plus_comm 1); auto.
+  rewrite <- Rdec.eqb_neq in H2. rewrite H2.
+  assert (Y <> X + Gamma g + 1).
+  1: apply gt_neq; auto.
+  rewrite <- Rdec.eqb_neq in H3. rewrite H3.
+  assert (Y <> X + Gamma g + Gamma h + 2).
+  1: { apply gt_neq; simpl in H. red; apply lt_le_trans with (X + Gamma g + Gamma h + 3).
+       apply plus_lt_compat_l; auto. rewrite (plus_assoc X) in H; rewrite <- (plus_assoc X); auto. }
+  rewrite <- Rdec.eqb_neq in H4. simpl in H4. rewrite H4.
+  apply IHd; red. transitivity (X + (Gamma (Recursion g h))); auto.
+  simpl. repeat rewrite <- plus_assoc; repeat apply plus_le_compat_l.
+  rewrite plus_comm; auto with arith.
++ red in H.
+  simpl; unfold RecVar_dec.
+  assert (Y <> X).
+  1: { apply gt_neq; red. apply lt_le_trans with (X + Gamma (Minimization h)); auto with arith. 
+       rewrite <- plus_0_r at 1. apply plus_lt_compat_l, Gamma_neq_zero. }
+  rewrite <- Rdec.eqb_neq in H0. rewrite H0.
+  assert (Y <> X + (@Gamma (S k) h) + 1).
+  1: { apply gt_neq; red. apply lt_le_trans with (X + (Gamma (Minimization h))); simpl; auto.
+       rewrite <- plus_assoc; apply plus_lt_compat_l. auto with arith. }
+  rewrite <- Rdec.eqb_neq in H1. rewrite H1.
+  apply IHd; red. transitivity (X + (Gamma (Minimization h))); auto.
+  simpl. repeat rewrite <- plus_assoc; repeat apply plus_le_compat_l.
+  rewrite plus_comm; auto with arith.
 Qed.
 
-Lemma converges_Implementation_aux_converges : forall {n} (f:PRFunction n) d Hd ps q i X Defs ns y,
+Theorem Implementation_converges : forall {n} (f:PRFunction n) ps q ns y,
+  ~In q ps -> converges f ns y -> 
+  forall (s:State), (forall H, s ps[@H] xx = ns[@H]) ->
+  exists c' tl, (Implementation f ps q, s) --[tl]-->* c' /\ Main (fst c') = End /\ snd c' q xx = y.
+Proof.
+intros.
+set (Hd := Nat.lt_succ_diag_r (depth f)).
+set (i := (S (max q (vmax ps)))).
+elim (Implementation_aux_converges f _ Hd ps q i 0 (Procedures (Implementation f ps q)) ns y H) with s; intros; auto.
++ destroy H2. rename x into s', x0 into tl.
+  simpl (0 + Gamma f) in H2.
+  elim (Call_reduce (Procedures (Implementation f ps q)) (Gamma f) s'); intros.
+  2: apply all_pids_not_nil.
+  rename x into tl'.
+  eexists. exists (tl++tl')%list; repeat split.
+  * eapply MCT_Trans; eauto.
+  * change (snd (Procedures (Implementation f ps q) (Gamma f)) = End).
+    apply Implementation_aux_ge; auto with arith.
+  * auto.
++ apply le_n_S. transitivity (vmax ps). apply vmax_In; auto. apply Nat.le_max_r.
++ apply le_n_S. apply Nat.le_max_l.
++ apply all_pids_not_nil.
+Qed.
+
+Lemma converges_Implementation_aux : forall {n} (f:PRFunction n) d Hd ps q i X Defs ns y,
   ~In q ps -> (forall p, In p ps -> p < i) -> q < i ->
   (forall Y, X <= Y < X + Gamma f -> fst (Defs Y) <> List.nil) ->
   (forall Y, X <= Y < X + Gamma f -> snd (Defs Y) = Implementation_aux f d Hd ps q i X Y) ->
@@ -1077,6 +654,28 @@ Lemma converges_Implementation_aux_converges : forall {n} (f:PRFunction n) d Hd 
   (Build_Program Defs (Call X),s) --[tl]-->* (Build_Program Defs (Call (X + Gamma f)),s')
   -> converges f ns y.
 (* Ugh *)
+Admitted.
+
+Theorem Implementation_diverges : forall {n} (f:PRFunction n) ps q ns,
+  ~In q ps -> diverges f ns -> 
+  forall (s:State), (forall H, s ps[@H] xx = ns[@H]) ->
+  forall c tl, (Implementation f ps q, s) --[tl]-->* c -> Main (fst c) <> End.
+Proof.
+intros.
+red; intro.
+set (Hd := Nat.lt_succ_diag_r (depth f)).
+set (i := (S (max q (vmax ps)))).
+induction c; induction a.
+simpl in H3; rewrite H3 in H2; clear Main0 H3. rename b into s'.
+elim (converges_Implementation_aux f _ Hd ps q i 0 (Procedures (Implementation f ps q)) ns (s' q xx) H) with s s' tl; intros; auto.
++ rewrite H0 in H3. inversion H3.
++ apply le_n_S. transitivity (vmax ps). apply vmax_In; auto. apply Nat.le_max_r.
++ apply le_n_S. apply Nat.le_max_l.
++ apply all_pids_not_nil.
++ 
+
+
+
 
 (*
 Fixpoint seq_compose {m} {k} (fs:t (PRFunction m) k) (ps:t Pid m) (target init:nat) (X:RecVar)
